BoC.lean
@@ -1,1 +1,2 @@
 import BoC.Semantics
+import BoC.Model
